Eliminate throw completly from actual implementation

IIO.ML.fst
@@ -5,21 +5,26 @@ open Common
 open IO.Free
 
 assume val ml_gettrace : args GetTrace -> ML (res GetTrace)
-assume val ml_openfile : args Openfile -> ML (res Openfile)
-assume val ml_read : args Read -> ML (res Read)
-assume val ml_close : args Close -> ML (res Close)
+assume val ml_openfile : args Openfile -> ML (io_res Openfile)
+assume val ml_read : args Read -> ML (io_res Read)
+assume val ml_close : args Close -> ML (io_res Close)
 
-val ml_io_all : (cmd:cmds) -> args cmd -> ML (res cmd)
-let ml_io_all cmd args =
+val ml_io_cmds : (cmd:io_cmds) -> args cmd -> ML (io_res cmd)
+let ml_io_cmds cmd args =
   match cmd with
-  | GetTrace -> ml_gettrace args
   | Openfile -> ml_openfile args
   | Read -> ml_read args
   | Close -> ml_close args
 
-
-val ml_io_execute : (cmd:cmds) -> args cmd -> ML (resm cmd)
-let ml_io_execute cmd argz =
+val ml_io_all : (cmd:io_cmds) -> args cmd -> ML (io_resm cmd)
+let ml_io_all cmd args =
   try_with
-    (fun _ -> Inl (ml_io_all cmd argz))
-    (fun err -> Inr err)
+    (fun _ -> (Inl (ml_io_cmds cmd args)) <: io_resm cmd)
+    (fun err -> (Inr err) <: io_resm cmd)
+
+
+val ml_io_execute : (cmd:cmds) -> args cmd -> ML (res cmd)
+let ml_io_execute cmd argz =
+  match cmd with
+  | GetTrace -> ml_gettrace argz
+  | _ -> ml_io_all cmd argz
