IIO.Effect.fst
@@ -4,7 +4,7 @@ open FStar.Tactics
 open ExtraTactics
 open FStar.Calc
 
-include Common
+open Common
 open IO.Free
 open IO.Effect
 open Hist
@@ -17,7 +17,7 @@ let rec iio_interpretation #a
   | Return x -> p x []
   (** internal_cmds **)
   | Call GetTrace args fnc ->
-    iio_interpretation (fnc (Inl h)) h p
+    iio_interpretation (fnc h) h p
   (** io_cmds **)
   | Call cmd args fnc -> (
     forall res. (
@@ -84,8 +84,8 @@ let lift_pure_iiowp
   (a:Type)
   (wp:pure_wp a)
   (f:(eqtype_as_type unit -> PURE a wp)) :
-  Tot (iio_irepr a (fun h p -> wp (fun r -> p (Inl r) [])))
-  = fun h p -> let r = elim_pure f (fun r -> p (Inl r) []) in iio_return _ r
+  Tot (iio_irepr a (fun h p -> wp (fun r -> p r [])))
+  = fun h p -> let r = elim_pure f (fun r -> p r []) in iio_return _ r
 
 sub_effect PURE ~> IIOwp = lift_pure_iiowp
 
@@ -144,12 +144,8 @@ let lift_iowp_iiowp (a:Type) (wp:hist a) (f:io_irepr a wp) :
 sub_effect IOwp ~> IIOwp = lift_iowp_iiowp
 
 let get_trace () : IIOwp trace
-  (fun h p -> forall r lt. r == (Inl h) /\ lt == [] ==>  p r lt) =
+  (fun h p -> forall lt. lt == [] ==>  p h lt) =
   IIOwp?.reflect (fun _ _ -> iio_call GetTrace ())
-
-let throw (#a:Type) (err:exn) : IIOwp a (fun _ p -> p (Inr err) []) =
-  IIOwp?.reflect(fun _ _ -> iio_throw a err)
-
 
 let iio_pre (pi : monitorable_prop) (h:trace) : Type0 =
   enforced_globally pi h
@@ -158,7 +154,7 @@ let iio_post
   (#a:Type)
   (pi : monitorable_prop)
   (h:trace)
-  (result:maybe a)
+  (result:a)
   (local_trace:trace) :
   Tot Type0 =
   enforced_globally pi (apply_changes h local_trace)
@@ -167,68 +163,11 @@ effect IIO
   (a:Type)
   (pi : monitorable_prop)
   (pre : trace -> Type0)
-  (post : trace -> maybe a -> trace -> Type0) =
+  (post : trace -> a -> trace -> Type0) =
   IIOwp a
     (fun h p ->
       pre h /\ iio_pre pi h /\
       (forall r lt. (iio_post pi h r lt /\ post h r lt) ==>  p r lt))
-
-let _IIOwp_as_IIO
-  (pre:'a -> trace -> bool)
-  (post:'a -> trace -> (m:maybe 'b) -> trace -> Type0)
-  (f:(x:'a ->
-    IIOwp 'b (fun h p -> pre x h /\ (forall r lt. post x h r lt ==> p r lt))))
-  (x:'a) :
-  IIOwp 'b (fun h p ->
-    (~(pre x h) ==> p (Inr Contract_failure) []) /\
-    (pre x h ==> (forall r lt. post x h r lt ==> p r lt))) =
-  let h = get_trace () in
-  if pre x h then f x
-  else IIO.Effect.throw Contract_failure
-
-let _IIOwp_as_IIO_2
-  (pre:'a -> 'b -> trace -> bool)
-  (post:'a -> 'b -> trace -> (m:maybe 'c) -> trace -> Type0)
-  (f:(x:'a -> y:'b ->
-    IIOwp 'c (fun h p -> pre x y h /\ (forall r lt. post x y h r lt ==> p r lt))))
-  (x:'a) (y:'b) :
-  IIOwp 'c (fun h p ->
-    (~(pre x y h) ==> p (Inr Contract_failure) []) /\
-    (pre x y h ==> (forall r lt. post x y h r lt ==> p r lt))) =
-  let h = get_trace () in
-  if pre x y h then f x y
-  else IIO.Effect.throw Contract_failure
-
-let _IIOwp_as_IIO_3
-  (pre:'a -> 'b -> 'c -> trace -> bool)
-  (post:'a -> 'b -> 'c -> trace -> (m:maybe 'd) -> trace -> Type0)
-  (f:(x:'a -> y:'b -> z:'c ->
-    IIOwp 'd (fun h p -> pre x y z h /\ (forall r lt. post x y z h r lt ==> p r lt))))
-  (x:'a) (y:'b) (z:'c) :
-  IIOwp 'd (fun h p ->
-    (~(pre x y z h) ==> p (Inr Contract_failure) []) /\
-    (pre x y z h ==> (forall r lt. post x y z h r lt ==> p r lt))) =
-  let h = get_trace () in
-  if pre x y z h then f x y z
-  else IIO.Effect.throw Contract_failure
-
-val dynamic_cmd :
-  (cmd : io_cmds) ->
-  (pi : monitorable_prop) ->
-  (arg : args cmd) ->
-  IIOwp (res cmd) (fun h p ->
-    (forall r lt.
-      ((match r with
-      | Inr Contract_failure -> lt == []
-      | _ -> lt == [convert_call_to_event cmd arg r]) /\
-      enforced_locally pi h lt) ==> p r lt))
-let dynamic_cmd (cmd:io_cmds) = _IIOwp_as_IIO_2 #monitorable_prop #(args cmd)
-  (fun pi (argz:args cmd) h -> pi h (| cmd, argz |))
-  (fun pi (argz:args cmd) h r lt ->
-      ~(Inr? r /\ Inr?.v r == Contract_failure) /\
-      lt == [convert_call_to_event cmd argz r] /\
-      enforced_locally pi h lt)
-  (static_cmd cmd)
 
 (** This tactic has the role to help F*/SMT to prove
 larger function bodies in the IIO Effect. This is
@@ -241,3 +180,63 @@ let iio_tactic () : Tac unit =
     let lem = pose_lemma (`(rev_append_rev_append ())) in
     norm [delta_only [`%iio_post;`%apply_changes]];
     explode ()
+
+let _IIOwp_as_IIO
+  (pre:'a -> trace -> bool)
+  (post:'a -> trace -> (m:'b) -> trace -> Type0)
+  (f:(x:'a ->
+    IIOwp 'b (fun h p -> pre x h /\ (forall r lt. post x h r lt ==> p r lt))))
+  (x:'a) :
+  IIOwp (maybe 'b) (fun h p ->
+    (~(pre x h) ==> p (Inr Contract_failure) []) /\
+    (pre x h ==> (forall r lt. post x h r lt ==> p (Inl r) lt)))
+    by (iio_tactic ()) =
+  let h = get_trace () in
+  if pre x h then (Inl (f x))
+  else (Inr Contract_failure)
+
+let _IIOwp_as_IIO_2
+  (pre:'a -> 'b -> trace -> bool)
+  (post:'a -> 'b -> trace -> (m:'c) -> trace -> Type0)
+  (f:(x:'a -> y:'b ->
+    IIOwp 'c (fun h p -> pre x y h /\ (forall r lt. post x y h r lt ==> p r lt))))
+  (x:'a) (y:'b) :
+  IIOwp (maybe 'c) (fun h p ->
+    (~(pre x y h) ==> p (Inr Contract_failure) []) /\
+    (pre x y h ==> (forall r lt. post x y h r lt ==> p (Inl r) lt)))
+    by (iio_tactic ()) =
+  let h = get_trace () in
+  if pre x y h then Inl (f x y)
+  else Inr Contract_failure
+
+let _IIOwp_as_IIO_3
+  (pre:'a -> 'b -> 'c -> trace -> bool)
+  (post:'a -> 'b -> 'c -> trace -> 'd -> trace -> Type0)
+  (f:(x:'a -> y:'b -> z:'c ->
+    IIOwp 'd (fun h p -> pre x y z h /\ (forall r lt. post x y z h r lt ==> p r lt))))
+  (x:'a) (y:'b) (z:'c) :
+  IIOwp (maybe 'd) (fun h p ->
+    (~(pre x y z h) ==> p (Inr Contract_failure) []) /\
+    (pre x y z h ==> (forall r lt. post x y z h r lt ==> p (Inl r) lt)))
+    by (iio_tactic ()) =
+  let h = get_trace () in
+  if pre x y z h then Inl (f x y z)
+  else Inr Contract_failure
+
+val dynamic_cmd :
+  (cmd : io_cmds) ->
+  (pi : monitorable_prop) ->
+  (arg : args cmd) ->
+  IIOwp (maybe (io_resm cmd)) (fun h p ->
+    (forall (r:maybe (io_resm cmd)) lt.
+      ((match r with
+      | Inr Contract_failure -> lt == []
+      | Inl r' -> lt == [convert_call_to_event cmd arg r']
+      | _ -> False) /\
+      enforced_locally pi h lt) ==> p r lt))
+let dynamic_cmd (cmd:io_cmds) = _IIOwp_as_IIO_2 #monitorable_prop #(args cmd)
+  (fun pi (argz:args cmd) h -> pi h (| cmd, argz |))
+  (fun pi (argz:args cmd) h r lt ->
+      lt == [convert_call_to_event cmd argz r] /\
+      enforced_locally pi h lt)
+  (static_cmd cmd)
